src/Contract.v
@@ -1,182 +1,503 @@
 Require Import Coq.Program.Basics.
 Require Import Coq.Program.Equality.
 Require Import Coq.Setoids.Setoid.
+Require Import Coq.Logic.Classical.
 
 Require Import FreeSpec.Program.
 Require Import FreeSpec.Interp.
+Require Import FreeSpec.Abstract.
 
 Record Contract
-       (I: Type -> Type) :=
-  { requirements {A: Type}
-                 (i: I A)
-    : Prop
-  ; promises {A: Type}
-             (i: I A)
-    : typeret i -> Prop
-  }.
+       (S: Type)
+       (I: Type -> Type)
+  :=
+    { abstract
+      : S
+    ; abstract_step {A: Type}
+                    (i: I A)
+      : S -> S
+    ; requirements {A: Type}
+      : I A -> S -> Prop
+    ; promises {A: Type}
+               (i: I A)
+      : typeret i -> S -> Prop
+    }.
 
-Arguments requirements [I] (c) [A] (i).
-Arguments promises [I] (c) [A] (i _).
+Arguments abstract [_ _] (_).
+Arguments abstract_step [_ _] (_) [_].
+Arguments requirements [_ _] (_) [_] (_ _).
+Arguments promises [_ _] (_) [_] (_ _).
 
-CoInductive Enforcer
-            {I: Type -> Type}
-            (c: Contract I)
-            (int: Interp I)
-  : Prop :=
-| enforced (Hprom: forall {A: Type}
-                          (i: I A),
-               requirements c i
-               -> (promises c i) (evalInstruction int i))
-           (Henf:  forall {A: Type}
-                          (i: I A),
-               requirements c i
-               -> Enforcer c (execInstruction int i))
-  : Enforcer c int.
+Definition set_abstract
+           {S: Type}
+           {I: Type -> Type}
+           (c: Contract S I)
+           (abs: S)
+  : Contract S I :=
+  {| abstract := abs
+   ; abstract_step := fun _ i' => abstract_step c i'
+   ; requirements := fun _ i' => requirements c i'
+   ; promises := fun _ i' => promises c i'
+  |}.
 
-Add Parametric Morphism
-    (I: Type -> Type)
-    (c: Contract I)
-  : (Enforcer c)
-    with signature (@interp_eq I) ==> (impl)
-      as enforcer_morphism.
-Proof.
-  cofix.
-  intros int int' Heq He.
-  constructor.
-  + intros A i Hreq.
-    rewrite <- Heq.
-    destruct He.
-    apply Hprom.
-    exact Hreq.
-  + intros A i Hreq.
-    destruct He.
-    apply Henf in Hreq.
-    apply (enforcer_morphism_Proper (execInstruction int i) (execInstruction int' i)) in Hreq.
-    ++ exact Hreq.
-    ++ destruct Heq.
-       apply Hnext.
-Qed.
+Definition contract_step
+           {S: Type}
+           {I: Type -> Type}
+           {A: Type}
+           (c: Contract S I)
+           (i: I A)
+  : Contract S I :=
+  {| abstract := abstract_step c i (abstract c)
+   ; abstract_step := fun _ i' => abstract_step c i'
+   ; requirements := fun _ i' => requirements c i'
+   ; promises := fun _ i' => promises c i'
+  |}.
 
-Inductive contractfull_program
-          {I: Type -> Type}
-          (c: Contract I)
-  : forall {A: Type}, Program I A -> Type :=
-| contractfull_instr {A: Type}
-                     (i: I A)
-                     (Hreq: requirements c i)
-  : contractfull_program c (instr i)
-| contractfull_ret {A: Type}
-                   (a: A)
-  : contractfull_program c (ret a)
-| contractfull_inv {A B: Type}
-                   (p: Program I A)
-                   (f: A -> Program I B)
-                   (Hcp: contractfull_program c p)
-                   (Hnext: forall (int: Interp I)
-                                  (Henf: Enforcer c int),
-                       contractfull_program c (f (evalProgram int p)))
-  : contractfull_program c (bind p f).
+Definition contract_derive
+           {S: Type}
+           {I: Type -> Type}
+           {A: Type}
+           (p: Program I A)
+           (int: Interp I)
+           (c: Contract S I)
+  : Contract S I :=
+  {| abstract := deriveAbstraction (abstract c) (abstract_step c) int p
+   ; abstract_step := fun _ i' => abstract_step c i'
+   ; requirements := fun _ i' => requirements c i'
+   ; promises := fun _ i' => promises c i'
+  |}.
 
-Lemma contractfull_instr_enforcement
+Lemma contract_derives_ret_eq
+      {S: Type}
       {I: Type -> Type}
       {A: Type}
-      {c: Contract I}
-      {i: I A}
-      {int: Interp I}
-      (Hc: contractfull_program c (instr i))
-      (Henf: Enforcer c int)
-  : Enforcer c (execProgram int (instr i)).
+      (a: A)
+      (int: Interp I)
+      (c: Contract S I)
+  : contract_derive (ret a) int c = c.
 Proof.
-  destruct Henf as [Hprom Henf].
-  apply (Henf A i).
-  inversion Hc; simpl_existT; subst.
+  induction c.
+  split.
+Qed.
+
+Lemma contract_derives_contract_step
+      {S: Type}
+      {I: Type -> Type}
+      {A: Type}
+      (i: I A)
+      (int: Interp I)
+      (c: Contract S I)
+  : contract_derive (instr i) int c = contract_step c i.
+Proof.
+  unfold contract_derive, contract_step.
+  reflexivity.
+Qed.
+
+CoInductive Enforcer
+            {S: Type}
+            {I: Type -> Type}
+            (int: Interp I)
+  : Contract S I -> Prop :=
+| enforced (c: Contract S I)
+           (Hprom: forall {A: Type}
+                          (i: I A),
+               requirements c i (abstract c)
+               -> (promises c i) (evalInstruction int i) (abstract c))
+           (Henf:  forall {A: Type}
+                          (i: I A),
+               requirements c i (abstract c)
+               -> Enforcer (execInstruction int i) (contract_step c i))
+  : Enforcer int c.
+
+Lemma enforcer_enforces_promises
+      {S: Type}
+      {I: Type -> Type}
+      {A: Type}
+      (i: I A)
+      (int: Interp I)
+      (c: Contract S I)
+      (Henf: Enforcer int c)
+      (Hreq: requirements c i (abstract c))
+  : promises c i (evalInstruction int i) (abstract c).
+Proof.
+  destruct Henf.
+  apply Hprom.
   exact Hreq.
 Qed.
 
-Lemma contractfull_ret_enforcement
-      {I: Type -> Type}
-      {A: Type}
-      {c: Contract I}
-      (a: A)
-      {int: Interp I}
-      (He: Enforcer c int)
-  : Enforcer c (execProgram int (ret a)).
-Proof.
-  exact He.
-Qed.
+Inductive contractfull_program
+          {S: Type}
+          {I: Type -> Type}
+          (c: Contract S I)
+  : forall {A: Type}, Program I A -> Prop :=
+| contractfull_instr {A: Type}
+                        (i: I A)
+                        (Hreq: requirements c i (abstract c))
+  : contractfull_program c (instr i)
+| tl_contractfull_ret {A: Type}
+                      (a: A)
+  : contractfull_program c (ret a)
+| tl_contractfull_inv {A B: Type}
+                      (p: Program I A)
+                      (f: A -> Program I B)
+                      (Hcp: contractfull_program c p)
+                      (Hnext: forall (int: Interp I)
+                                     (Henf: Enforcer int c),
+                          contractfull_program (contract_derive p int c) (f (evalProgram int p)))
+  : contractfull_program c (bind p f).
 
-Lemma contractfull_program_enforcement
+Lemma contractfull_program_bind_ret
+      {S: Type}
       {I: Type -> Type}
       {A B: Type}
-      (c: Contract I)
+      (a: A)
+      (f: A -> Program I B)
+      (c: Contract S I)
+  : contractfull_program c (f a) -> contractfull_program c (bind (ret a) f).
+Proof.
+  intros Hp.
+  constructor.
+  + constructor.
+  + intros int Henf.
+    cbn.
+    rewrite contract_derives_ret_eq.
+    exact Hp.
+Qed.
+
+Conjecture contractfull_program_bind_ret'
+  : forall {S: Type}
+           {I: Type -> Type}
+           {A B: Type}
+           (a: A)
+           (f: A -> Program I B)
+           (c: Contract S I),
+    contractfull_program c (bind (ret a) f) -> contractfull_program c (f a).
+
+Lemma enforcer_instruction_contractfull_enforcer
+      {S: Type}
+      {I: Type -> Type}
+      {A: Type}
+      (i: I A)
+      (int: Interp I)
+      (c: Contract S I)
+      (H: Enforcer int c)
+      (Hp: contractfull_program c (instr i))
+  : Enforcer (abstractExec (abstract c) (abstract_step c) int (instr i)) (contract_derive (instr i) int c).
+Proof.
+  cbn.
+  constructor.
+  + intros B i' Hinst.
+    destruct H as [c Hprom Henf].
+    inversion Hp.
+    apply Henf in Hreq.
+    apply inj_pair2 in H1.
+    subst.
+    inversion Hreq.
+    rewrite contract_derives_contract_step.
+    apply Hprom0.
+    exact Hinst.
+  + intros B i' Hinst.
+    destruct H as [c Hprom Henf].
+    inversion Hp.
+    apply Henf in Hreq.
+    apply inj_pair2 in H1.
+    subst.
+    inversion Hreq.
+    rewrite contract_derives_contract_step.
+    apply Henf0.
+    exact Hinst.
+Qed.
+
+Lemma enforcer_ret_contractfull_enforcer
+      {S: Type}
+      {I: Type -> Type}
+      {A: Type}
+      (a: A)
+      (int: Interp I)
+      (c: Contract S I)
+      (H: Enforcer int c)
+  : Enforcer (abstractExec (abstract c) (abstract_step c) int (ret a)) (contract_derive (ret a) int c).
+Proof.
+  rewrite (contract_derives_ret_eq a int c).
+  unfold abstractExec.
+  cbn.
+  exact H.
+Qed.
+
+Lemma contract_derive_assoc
+      {S: Type}
+      {I: Type -> Type}
+      {A B C: Type}
       (p: Program I A)
-  : forall (int: Interp I)
-           (Hc: contractfull_program c p)
-           (He: Enforcer c int),
-    Enforcer c (execProgram int p).
+      (f: A -> Program I B)
+      (f': B -> Program I C)
+      (int: Interp I)
+      (c: Contract S I)
+  : contract_derive (bind (bind p f) f') int c
+    = contract_derive (bind p (fun x => bind (f x) f')) int c.
+Proof.
+  reflexivity.
+Qed.
+
+Lemma exec_program_assoc'
+      {S: Type}
+      {I: Type -> Type}
+      {A: Type}
+      (p: Program I A)
+  : forall {B C: Type}
+           (f: A -> Program I B)
+           (f': B -> Program I C)
+           (int: Interp I),
+    execProgram int (bind (bind p f) f')
+    = execProgram int (bind p (fun x => (bind (f x) f'))).
+Proof.
+  intros B C f f' int.
+  reflexivity.
+Qed.
+
+Lemma exec_abs_assoc
+      {S: Type}
+      {I: Type -> Type}
+      {A: Type}
+      (p: Program I A)
+  : forall {B: Type}
+           (f: A -> Program I B)
+           (int: Interp I)
+           (c: Contract S I),
+    abstractExec (abstract c) (abstract_step c) int (bind p f)
+    = abstractExec (abstract (contract_derive p int c))
+                   (abstract_step (contract_derive p int c))
+                   (abstractExec (abstract c) (abstract_step c) int p)
+                   (f (evalProgram int p)).
+Proof.
+  intros B f int c.
+  repeat rewrite abstract_exec_exec_program_same.
+  reflexivity.
+Qed.
+
+Lemma eval_program_assoc
+      {S: Type}
+      {I: Type -> Type}
+      {A: Type}
+      (p: Program I A)
+  : forall {B: Type}
+           (f: A -> Program I B)
+           (int: Interp I)
+           (c: Contract S I),
+    evalProgram int (bind p f)
+    = evalProgram (abstractExec (abstract c) (abstract_step c) int p)
+                  (f (evalProgram int p)).
+Proof.
+  intros B f int c.
+  rewrite abstract_exec_exec_program_same.
+  reflexivity.
+Qed.
+
+Lemma contract_derive_bind
+      {S: Type}
+      {I: Type -> Type}
+      {A: Type}
+      (p: Program I A)
+  : forall {B: Type}
+           (f: A -> Program I B)
+           (int: Interp I)
+           (c: Contract S I),
+    contract_derive (f (evalProgram int p))
+                    (abstractExec (abstract c) (abstract_step c) int p) (contract_derive p int c)
+    = contract_derive (bind p f) int c.
 Proof.
   induction p.
-  + intros int Hc He.
-    apply (contractfull_ret_enforcement a He).
-  + intros int Hc He.
-    apply (contractfull_instr_enforcement Hc He).
-  + intros int Hc He.
-    assert (contractfull_program c (f (evalProgram int p))) as Hc'.
-    ++ inversion Hc; repeat simpl_existT; subst.
-       apply (Hnext int He).
-    ++ inversion Hc; repeat simpl_existT; subst.
-       apply H with (int:=execProgram int p) in Hc'.
-       exact Hc'.
-       apply IHp.
-       +++ exact Hcp.
-       +++ exact He.
+  + reflexivity.
+  + reflexivity.
+  + intros C f' int' c'.
+    rewrite contract_derive_assoc.
+    rewrite <- (IHp C) .
+    rewrite <- H.
+    rewrite <- eval_program_assoc.
+    rewrite <- exec_abs_assoc.
+    rewrite <- (IHp A) .
+    reflexivity.
+Qed.
+
+Lemma abstractExec_bind
+      {S: Type}
+      {I: Type -> Type}
+      {A B: Type}
+      (p: Program I A)
+  : forall (f: A -> Program I B)
+           (int: Interp I)
+           (c: Contract S I),
+    abstractExec (abstract (contract_derive p int c))
+                 (abstract_step (contract_derive p int c))
+                 (abstractExec (abstract c)
+                               (abstract_step c)
+                               int
+                               p)
+                 (f (evalProgram int p))
+    = abstractExec (abstract c) (abstract_step c) int (bind p f).
+Proof.
+  intros f int c.
+  repeat rewrite abstract_exec_exec_program_same.
+  reflexivity.
+Qed.
+
+Lemma enforcer_contractfull_enforcer
+      {S: Type}
+      {I: Type -> Type}
+      {A: Type}
+      (p: Program I A)
+  : forall (c: Contract S I)
+           (int: Interp I)
+           (H: Enforcer int c)
+           (Hp: contractfull_program c p),
+    Enforcer (abstractExec (abstract c) (abstract_step c) int p) (contract_derive p int c).
+Proof.
+  induction p.
+  + intros c int He Hp;
+      apply (enforcer_ret_contractfull_enforcer a int c He).
+  + intros c int He Hp;
+      apply (enforcer_instruction_contractfull_enforcer i int c He Hp).
+  + intros c int He Hp.
+    inversion Hp;
+      apply inj_pair2 in H3;
+      repeat apply inj_pair2 in H4;
+      subst.
+    apply (IHp c int He) in Hcp.
+    rewrite <- abstractExec_bind.
+    rewrite <- contract_derive_bind.
+    apply H.
+    ++ exact Hcp.
+    ++ apply Hnext.
+       exact He.
 Qed.
 
 Definition contract_preserves_inv
-            {I: Type -> Type}
-            {State: Type}
-            (c: Contract I)
-            (inv: State -> Prop)
-            (step: PS State)
+           {S: Type}
+           {I: Type -> Type}
+           {State: Type}
+           (requirements: forall (R: Type), I R -> S -> Prop)
+           (abs_step: forall (R: Type), I R -> S -> S)
+           (inv: S -> State -> Prop)
+           (step: @PS I State)
   := forall {A: Type}
             (i: I A)
+            (abs: S)
             (s: State),
-     inv s
-     -> requirements c i
-     -> inv (snd (step A s i)).
+    inv abs s
+    -> requirements A i abs
+    -> inv (abs_step A i abs) (snd (step A s i)).
 
-Definition contract_enforces_promises
-            {I: Type -> Type}
-            {State: Type}
-            (c: Contract I)
-            (inv: State -> Prop)
-            (step: PS State)
-  := forall {A: Type}
-            (i: I A)
-            (s: State),
-    inv s
-    -> requirements c i
-    -> promises c i (fst (step A s i)).
-
-Lemma stateful_contract_enforcement
+Lemma contract_preserves_inv_propagates
+      {S: Type}
       {I: Type -> Type}
       {State: Type}
-      (c: Contract I)
-      (inv: State -> Prop)
-      (step: PS State)
-      (Hpres: contract_preserves_inv c inv step)
-      (Henf: contract_enforces_promises c inv step)
-  : forall (s: State)
-  , inv s
-    -> Enforcer c (mkInterp step s).
+      (inv: S -> State -> Prop)
+      (step: @PS I State)
+  : forall {A: Type}
+           (c: Contract S I)
+           (i: I A),
+    contract_preserves_inv (requirements c) (abstract_step c) inv step
+    -> requirements c i (abstract c)
+    -> contract_preserves_inv (requirements (contract_step c i)) (abstract_step (contract_step c i)) inv step.
+Proof.
+  intros A c i Hpres Hreq.
+  unfold contract_preserves_inv in *.
+  intros B i' s Hinv Hreq'.
+  apply Hpres.
+  exact Hreq'.
+Qed.
+
+Definition contract_enforces_promises
+           {S: Type}
+           {I: Type -> Type}
+           {State: Type}
+           (requirements: forall (R: Type), I R -> S -> Prop)
+           (promises: forall {R: Type} (i: I R), typeret i -> S -> Prop)
+           (abs_step: forall (R: Type), I R -> S -> S)
+           (inv: S -> State -> Prop)
+           (step: @PS I State)
+  := forall {A: Type}
+            (i: I A)
+            (s: State)
+            (abs: S),
+    inv abs s
+    -> requirements A i abs
+    -> promises i (fst (step A s i)) abs.
+
+Lemma contract_enforces_promises_propagates
+      {S: Type}
+      {I: Type -> Type}
+      {State: Type}
+      (c: Contract S I)
+      (inv: S -> State -> Prop)
+      (step: @PS I State)
+  : forall {A: Type}
+           (i: I A),
+    contract_enforces_promises (requirements c) (promises c) (abstract_step c) inv step
+    -> requirements c i (abstract c)
+    -> contract_enforces_promises (requirements (contract_step c i))
+                                  (promises (contract_step c i))
+                                  (abstract_step (contract_step c i)) inv step.
+Proof.
+  intros A i Henf Hreq.
+  unfold contract_enforces_promises in *.
+  intros B i' s abs Hinv Hreq'.
+  cbn.
+  apply Henf.
+  + exact Hinv.
+  + exact Hreq'.
+Qed.
+
+Fact _stateful_contract_enforcement
+     {S: Type}
+     {I: Type -> Type}
+     {State: Type}
+     (c: Contract S I)
+     (inv: S -> State -> Prop)
+     (step: @PS I State)
+  : forall (abs: S)
+           (Hpres: contract_preserves_inv (requirements c) (abstract_step c) inv step)
+           (Henf: contract_enforces_promises (requirements c) (promises c) (abstract_step c) inv step)
+           (s: State),
+    inv abs s
+    -> Enforcer (mkInterp step s) (set_abstract c abs).
 Proof.
   cofix.
-  intros s Hinv.
+  intros abs Hpres Henf s Hinv .
   constructor.
   + intros A i Hreq.
-    apply (Henf A i s Hinv Hreq).
+    unfold contract_enforces_promises in Henf.
+    cbn in *.
+    apply (Henf A i s abs Hinv Hreq).
   + intros A i Hreq.
-    apply (Hpres A i s) in Hinv.
-    ++ apply (stateful_contract_enforcement (snd (step A s i)) Hinv).
-    ++ exact Hreq.
+    apply _stateful_contract_enforcement.
+    ++ apply  Hpres.
+    ++ apply  Henf.
+    ++ cbn in *.
+       apply (contract_preserves_inv_propagates inv step (set_abstract c abs) i Hpres Hreq A i abs s).
+       +++ apply Hinv.
+       +++ exact Hreq.
+Qed.
+
+Lemma stateful_contract_enforcement
+      {S: Type}
+      {I: Type -> Type}
+      {State: Type}
+      (c: Contract S I)
+      (inv: S -> State -> Prop)
+      (step: @PS I State)
+      (Hpres: contract_preserves_inv (requirements c) (abstract_step c) inv step)
+      (Henf: contract_enforces_promises (requirements c) (promises c) (abstract_step c) inv step)
+  : forall (s: State),
+    inv (abstract c) s
+    -> Enforcer (mkInterp step s) c.
+Proof.
+  intros s Hinv.
+  cbn.
+  assert (set_abstract c (abstract c) = c)
+    as Heq
+      by (induction c;
+          reflexivity).
+  rewrite <- Heq.
+  apply (_stateful_contract_enforcement c inv step (abstract c) Hpres Henf s Hinv).
 Qed.
