src/Abstract.v
@@ -1,0 +1,111 @@
+Require Import FreeSpec.Program.
+Require Import FreeSpec.Interp.
+
+(** In this library, we provide the functions to
+
+ *)
+
+Fixpoint abstractRun
+         {S: Type}
+         {I: Type -> Type}
+         {A: Type}
+         (abs: S)
+         (abs_step: forall (R:Type), I R -> S -> S)
+         (int: Interp I)
+         (p: Program I A)
+  : (A * (Interp I) * S) :=
+  match p with
+  | ret a => (a, int, abs)
+  | instr i => (evalInstruction int i,
+                execInstruction int i,
+                abs_step _ i abs)
+  | bind p' f => abstractRun (snd (abstractRun abs abs_step int p'))
+                             abs_step
+                             (snd (fst (abstractRun abs abs_step int p')))
+                             (f (fst (fst (abstractRun abs abs_step int p' ))))
+  end.
+
+(** Similary to [FreeSpec.Program.runProgram]
+
+ *)
+
+Definition abstractExec
+           {S: Type}
+           {I: Type -> Type}
+           {A: Type}
+           (abs: S)
+           (abs_step: forall (R:Type), I R -> S -> S)
+           (int: Interp I)
+           (p: Program I A)
+  : Interp I :=
+  snd (fst (abstractRun abs abs_step int p)).
+
+Definition abstractEval
+           {S: Type}
+           {I: Type -> Type}
+           {A: Type}
+           (abs: S)
+           (abs_step: forall (R:Type), I R -> S -> S)
+           (int: Interp I)
+           (p: Program I A)
+  : A :=
+  fst (fst (abstractRun abs abs_step int p)).
+
+Definition deriveAbstraction
+           {S: Type}
+           {I: Type -> Type}
+           {A: Type}
+           (abs: S)
+           (abs_step: forall (R: Type), I R -> S -> S)
+           (int: Interp I)
+           (p: Program I A)
+  : S :=
+  snd (abstractRun abs abs_step int p).
+
+Lemma abstract_run_run_program_same
+      {S: Type}
+      {I: Type -> Type}
+      {A: Type}
+  : forall (p: Program I A)
+           (abs: S)
+           (abs_step: forall (R: Type), I R -> S -> S)
+           (int: Interp I),
+    fst (abstractRun abs abs_step int p) = runProgram int p.
+Proof.
+  induction p; intros abs abs_step int; cbn.
+  + reflexivity.
+  + apply injective_projections; reflexivity.
+  + rewrite H; rewrite IHp; reflexivity.
+Qed.
+
+Lemma abstract_eval_eval_program_same
+      {S: Type}
+      {I: Type -> Type}
+      {A: Type}
+  : forall (p: Program I A)
+           (abs: S)
+           (abs_step: forall (R: Type), I R -> S -> S)
+           (int: Interp I),
+    abstractEval abs abs_step int p = evalProgram int p.
+Proof.
+  intros p abs abs_step int.
+  unfold abstractEval, evalProgram.
+  rewrite abstract_run_run_program_same.
+  reflexivity.
+Qed.
+
+Lemma abstract_exec_exec_program_same
+      {S: Type}
+      {I: Type -> Type}
+      {A: Type}
+  : forall (p: Program I A)
+           (abs: S)
+           (abs_step: forall (R: Type), I R -> S -> S)
+           (int: Interp I),
+    abstractExec abs abs_step int p = execProgram int p.
+Proof.
+  intros p abs abs_step int.
+  unfold abstractExec, execProgram.
+  rewrite abstract_run_run_program_same.
+  reflexivity.
+Qed.
