src/Contract/Constant.v
@@ -1,0 +1,116 @@
+Require Import FreeSpec.Interp.
+Require Import FreeSpec.Contract.
+
+Definition const_contract_requirements
+           {I: Interface}
+           (requirements: forall (A: Type), I A -> Prop)
+  := fun {A: Type} (i: I A) (_: unit) => requirements A i.
+
+Definition const_contract_promises
+           {I: Interface}
+           (promises: forall (A: Type)
+                             (i: I A),
+               typeret i -> Prop)
+  := fun {A: Type} (i: I A) (a: A) (_: unit) => promises A i a.
+
+Definition constant_contract
+           {I: Interface}
+           (requirements: forall (A: Type), I A -> Prop)
+           (promises: forall (A: Type)
+                             (i: I A),
+               typeret i -> Prop)
+  : Contract unit I :=
+  {| abstract := tt
+   ; abstract_step := fun (A: Type) (_: I A) (x: unit) => x
+   ; requirements := @const_contract_requirements I requirements
+   ; promises := @const_contract_promises I promises
+   |}.
+
+Definition requirements_preserves_inv
+           {I: Interface}
+           {State: Type}
+           (requirements: forall (A: Type), I A -> Prop)
+           (step: @PS I State)
+           (inv: State -> Prop)
+  := forall {A: Type}
+            (i: I A)
+            (s: State),
+    inv s
+    -> requirements A i
+    -> inv (snd (step A s i)).
+
+Lemma const_contract_preserves_inv
+      {I: Interface}
+      {State: Type}
+      (requirements: forall (A: Type), I A -> Prop)
+      (step: @PS I State)
+      (inv: State -> Prop)
+  : requirements_preserves_inv requirements step inv
+    -> contract_preserves_inv (@const_contract_requirements I requirements)
+                              (fun _ _ _ => tt)
+                              (fun _ s => inv s)
+                              step.
+Proof.
+  unfold requirements_preserves_inv, contract_preserves_inv.
+  intros Hreq.
+  intros B i _s s Hinv Hconst.
+  apply (Hreq B i s Hinv Hconst).
+Qed.
+
+Definition requirements_brings_promises
+           {I: Interface}
+           {State: Type}
+           (requirements: forall (A: Type), I A -> Prop)
+           (promises: forall (A: Type), I A -> A -> Prop)
+           (step: @PS I State)
+           (inv: State -> Prop)
+  := forall {A: Type}
+            (i: I A)
+            (s: State),
+    inv s
+    -> requirements A i
+    -> promises A i (fst (step A s i)).
+
+Lemma const_contract_enforces_promises
+      {I: Interface}
+      {State: Type}
+      (requirements: forall (A: Type), I A -> Prop)
+      (promises: forall (A: Type), I A -> A -> Prop)
+      (step: @PS I State)
+      (inv: State -> Prop)
+  : requirements_brings_promises requirements promises step inv
+    -> contract_enforces_promises (@const_contract_requirements I requirements)
+                                  (@const_contract_promises I promises)
+                                  (fun _ _ _ => tt)
+                                  (fun _ s => inv s)
+                                  step.
+Proof.
+  unfold requirements_brings_promises, contract_enforces_promises.
+  intros Hreq.
+  intros B i s _s Hinv Hconst.
+  apply (Hreq B i s Hinv Hconst).
+Qed.
+
+Lemma const_contract_enforcement
+      {I: Interface}
+      {State: Type}
+      (requirements: forall (A: Type), I A -> Prop)
+      (promises: forall (A: Type), I A -> A -> Prop)
+      (step: @PS I State)
+      (inv: State -> Prop)
+      (Hpres: requirements_preserves_inv requirements step inv)
+      (Henf: requirements_brings_promises requirements promises step inv)
+  : forall (s: State),
+    inv s
+    -> Enforcer (mkInterp step s) (constant_contract requirements promises).
+Proof.
+  intros s Hinv.
+  apply (stateful_contract_enforcement (constant_contract requirements promises)
+                                       (fun _ s => inv s)
+                                       step).
+  + apply const_contract_preserves_inv.
+    exact Hpres.
+  + apply const_contract_enforces_promises.
+    exact Henf.
+  + exact Hinv.
+Qed.
