src/Contract/Temporal.v
@@ -1,0 +1,114 @@
+Require Import FreeSpec.Interp.
+Require Import FreeSpec.Contract.
+Require Import FreeSpec.TemporalLogic.
+Require Import FreeSpec.Contract.
+
+Definition temporal_step (I: Interface) :=
+  fun (R: Type) (i: I R) => tl_step (instruction i).
+
+Definition temporal_requirements (I: Interface) :=
+  fun (R: Type) (i: I R) => instruction_satisfies (instruction i).
+
+Definition temporal_contract
+           {I: Interface}
+           (tl: Formula (ISet I))
+           (promises: forall (R: Type)
+                             (i: I R),
+               typeret i -> Formula (ISet I) -> Prop)
+  : Contract (Formula (ISet I)) I :=
+  {| abstract := tl
+   ; abstract_step := temporal_step I
+   ; requirements := temporal_requirements I
+   ; promises := fun (R: Type) => @promises R
+   |}.
+
+Definition temporal_requirements_preserves_inv
+           {I: Interface}
+           {State: Type}
+           (step: @PS I State)
+           (inv: Formula (ISet I) -> State -> Prop)
+  := forall {A: Type}
+            (i: I A)
+            (s: State)
+            (tl: Formula (ISet I)),
+    inv tl s
+    -> instruction_satisfies (instruction i) tl
+    -> inv (tl_step (instruction i) tl) (snd (step A s i)).
+
+Lemma temporal_contract_preserves_inv
+      {I: Interface}
+      {State: Type}
+      (step: @PS I State)
+      (inv: Formula (ISet I) -> State -> Prop)
+  : temporal_requirements_preserves_inv step inv
+    -> contract_preserves_inv (temporal_requirements I)
+                              (temporal_step I)
+                              inv
+                              step.
+Proof.
+  unfold temporal_requirements_preserves_inv, contract_preserves_inv.
+  intros Hreq B i tl s Hinv Hsatisfies.
+  apply (Hreq B i s tl Hinv Hsatisfies).
+Qed.
+
+Definition temporal_requirements_enforces_promises
+           {I: Interface}
+           {State: Type}
+           (step: @PS I State)
+           (inv: Formula (ISet I) -> State -> Prop)
+           (promises: forall (R: Type)
+                             (i: I R),
+               typeret i -> Formula (ISet I) -> Prop)
+  := forall {A: Type}
+            (i: I A)
+            (s: State)
+            (tl: Formula (ISet I)),
+    inv tl s
+    -> instruction_satisfies (instruction i) tl
+    -> promises A i (fst (step A s i)) tl.
+
+Lemma temporal_contract_enforces_promises
+      {I: Interface}
+      {State: Type}
+      (step: @PS I State)
+      (inv: Formula (ISet I) -> State -> Prop)
+      (promises: forall (R: Type)
+                        (i: I R),
+          typeret i -> Formula (ISet I) -> Prop)
+  : temporal_requirements_enforces_promises step inv promises
+    -> contract_enforces_promises (temporal_requirements I)
+                                  promises
+                                  (temporal_step I)
+                                  inv
+                                  step.
+Proof.
+  unfold temporal_requirements_enforces_promises, contract_enforces_promises.
+  intros Hreq B i tl s Hinv Hsatisfies.
+  apply (Hreq B i tl s Hinv Hsatisfies).
+Qed.
+
+Lemma temporal_contract_enforcement
+      {I: Interface}
+      {State: Type}
+      (step: @PS I State)
+      (inv: Formula (ISet I) -> State -> Prop)
+      (promises: forall (R: Type)
+                        (i: I R),
+          typeret i -> Formula (ISet I) -> Prop)
+      (tl: Formula (ISet I))
+      (Hpres: temporal_requirements_preserves_inv step inv)
+      (Henf: temporal_requirements_enforces_promises step inv promises)
+  : forall (s: State),
+    inv tl s
+    -> Enforcer (mkInterp step s) (temporal_contract tl promises).
+Proof.
+  intros s Hinv.
+  apply (stateful_contract_enforcement (temporal_contract tl promises)
+                                       inv
+                                       step).
+  + apply temporal_contract_preserves_inv.
+    exact Hpres.
+  + apply temporal_contract_enforces_promises.
+    exact Henf.
+  + exact Hinv.
+Qed.
